Cleaned up random elixir files and renamed michael_formal to formal

formal/EFSM.thy
@@ -1,58 +1,328 @@
+subsection \<open>Extended Finite State Machines\<close>
+text\<open>
+This theory defines extended finite state machines. Each EFSM takes a type variable which represents
+$S$. This is a slight devaition from the definition presented in \cite{foster2018} as this
+type variable may be of an infinite type such as integers, however the intended use is for custom
+finite types. See the examples for details.
+\<close>
+
 theory EFSM
-imports IO
+  imports "~~/src/HOL/Library/FSet" Transition FSet_Utils
 begin
 
-fun map_or_empty :: "('a, 'b list) map \<Rightarrow> 'a \<Rightarrow> 'b list" where
-"map_or_empty m x = 
-    (case m(x) of
-      None \<Rightarrow> []
-     |  Some ls \<Rightarrow> ls)"
+type_synonym label = string
+type_synonym arity = nat
+type_synonym inputs = "value list"
+type_synonym outputs = "value option list"
+type_synonym updates = "update_function list"
+type_synonym event = "(label \<times> inputs)"
+type_synonym trace = "event list"
+type_synonym observation = "outputs list"
 
-abbreviation is_possible_step :: "efsm \<Rightarrow> statename \<Rightarrow> statename \<Rightarrow> transition \<Rightarrow> label \<Rightarrow> inputs \<Rightarrow> data \<Rightarrow> bool" where
-"is_possible_step e s s' t l ip dt \<equiv> 
-  (((label t) = l) \<and> (find (\<lambda>x . x = t) (map_or_empty (M e) (s,s')) \<noteq> None) \<and> (guard t)(ip,dt))"
+type_synonym transition_matrix = "((nat \<times> nat) \<times> transition) fset"
 
-abbreviation possible_steps :: "efsm \<Rightarrow> statename \<Rightarrow> label \<Rightarrow> inputs \<Rightarrow> data \<Rightarrow> (statename * transition) list" where
-"possible_steps e s l ip dt \<equiv> [(s',t) . s' \<leftarrow> S e, t \<leftarrow> (map_or_empty (M e) (s,s')), is_possible_step e s s' t l ip dt]"
+primrec input2state :: "value list \<Rightarrow> nat \<Rightarrow> datastate" where
+  "input2state [] _ = <>" |
+  "input2state (h#t) i = (\<lambda>x. if x = I i then Some h else (input2state t (i+1)) x)"
 
-definition step :: "efsm \<Rightarrow> statename \<Rightarrow> label \<Rightarrow> inputs \<Rightarrow> data \<Rightarrow> (statename \<times> outvalues \<times> data) option" where
-"step e s l ip dt \<equiv>
-  case possible_steps e s l ip dt of
-    [] \<Rightarrow> None
-    | [(s',t)] \<Rightarrow> Some (s', (outputs t) (ip,dt), (updates t) (ip,dt))
-    | _ \<Rightarrow> None"
-declare step_def [simp]
+lemma hd_input2state: "length i \<ge> 1 \<Longrightarrow> input2state i 1 (I 1) = Some (hd i)"
+  by (metis hd_Cons_tl input2state.simps(2) le_numeral_extra(2) length_0_conv)
 
-primrec observe_steps :: "efsm \<Rightarrow> statename \<Rightarrow> data \<Rightarrow> trace \<Rightarrow> observation" where
- "observe_steps _ _ _ [] = []"
-|"observe_steps e s dt (ip#ips) = 
-    (case step e s (fst ip) (snd ip) dt of
-        Some (s', ops, dt') \<Rightarrow> ops#(observe_steps e s' dt' ips)
-      | None                \<Rightarrow> []
+definition join_ir :: "value list \<Rightarrow> datastate \<Rightarrow> datastate" where
+  "join_ir i r \<equiv> (\<lambda>x. case x of
+    R n \<Rightarrow> r (R n) |
+    I n \<Rightarrow> (input2state i 1) (I n)
+  )"
+declare join_ir_def [simp]
+
+definition S :: "transition_matrix \<Rightarrow> nat fset" where
+  "S m = (fimage (\<lambda>((s, s'), t). s) m) |\<union>| fimage (\<lambda>((s, s'), t). s') m"
+
+primrec apply_outputs :: "output_function list \<Rightarrow> datastate \<Rightarrow> outputs" where
+  "apply_outputs [] _ = []" |
+  "apply_outputs (h#t) s = (aval h s)#(apply_outputs t s)"
+
+primrec apply_guards :: "guard list \<Rightarrow> datastate \<Rightarrow> bool" where
+  "apply_guards [] _ = True" |
+  "apply_guards (h#t) s =  ((gval h s) = Some True \<and> (apply_guards t s))"
+
+primrec apply_updates :: "(vname \<times> aexp) list \<Rightarrow> datastate \<Rightarrow> datastate \<Rightarrow> datastate" where
+  "apply_updates [] _ new = new" |
+  "apply_updates (h#t) old new = (\<lambda>x. if x = (fst h) then (aval (snd h) old) else (apply_updates t old new) x)"
+
+definition possible_steps :: "transition_matrix \<Rightarrow> nat \<Rightarrow> datastate \<Rightarrow> label \<Rightarrow> inputs \<Rightarrow> (nat \<times> transition) fset" where
+  "possible_steps e s r l i = fimage (\<lambda>((origin, dest), t). (dest, t)) (ffilter (\<lambda>((origin, dest::nat), t::transition). origin = s \<and> (Label t) = l \<and> (length i) = (Arity t) \<and> apply_guards (Guard t) (join_ir i r)) e)"
+
+definition step :: "transition_matrix \<Rightarrow> nat \<Rightarrow> datastate \<Rightarrow> label \<Rightarrow> inputs \<Rightarrow> (transition \<times> nat \<times> outputs \<times> datastate) option" where
+"step e s r l i =
+(if fis_singleton (possible_steps e s r l i) then (let (s', t) =  (fthe_elem (possible_steps e s r l i)) in Some (t, s', (apply_outputs (Outputs t) (join_ir i r)), (apply_updates (Updates t) (join_ir i r) r))) else None)"
+
+lemma step_empty[simp]:"step {||} s r l i = None"
+proof-
+  have ffilter_empty: "ffilter
+       (\<lambda>((origin, dest), t).
+           origin = s \<and>
+           Label t = l \<and> length i = Arity t \<and> apply_guards (Guard t) (case_vname (\<lambda>n. input2state i 1 (I n)) (\<lambda>n. r (R n))))
+       {||} = {||}"
+    by auto
+  show ?thesis
+    by (simp add: step_def possible_steps_def ffilter_empty)
+qed
+
+primrec observe_all :: "transition_matrix \<Rightarrow> nat \<Rightarrow> datastate \<Rightarrow> trace \<Rightarrow> (transition \<times> nat \<times> outputs \<times> datastate) list" where
+  "observe_all _ _ _ [] = []" |
+  "observe_all e s r (h#t) =
+    (case (step e s r (fst h) (snd h)) of
+      (Some (transition, s', outputs, updated)) \<Rightarrow> (((transition, s', outputs, updated)#(observe_all e s' updated t))) |
+      _ \<Rightarrow> []
     )"
-declare observe_steps_def [simp]
 
-primrec pairs :: "statename list \<Rightarrow> statename \<Rightarrow> (statename \<times> statename) list" where
-  "pairs [] _ = []"
-|"pairs (h#t) x = (if x = h then (h, x)#(pairs t x) else (h, x)#(x, h)#(pairs t x))"
+definition state :: "(transition \<times> nat \<times> outputs \<times> datastate) \<Rightarrow> nat" where
+  "state x \<equiv> fst (snd x)"
 
-primrec allPairs :: "statename list \<Rightarrow> (statename \<times> statename) list" where
-  "allPairs [] = []"
-| "allPairs (h#t) = (pairs (h#t) h)@(allPairs t)"
+definition observe_trace :: "transition_matrix \<Rightarrow> nat \<Rightarrow> datastate \<Rightarrow> trace \<Rightarrow> observation" where
+  "observe_trace e s r t \<equiv> map (\<lambda>(t,x,y,z). y) (observe_all e s r t)"
 
-definition observe :: "efsm \<Rightarrow> trace \<Rightarrow> observation" where
-"observe e tr \<equiv> observe_steps e (s0 e) blankdata tr"
+lemma observe_empty: "t = [] \<Longrightarrow> observe_trace e 0 <> t = []"
+  by (simp add: observe_trace_def)
 
-definition equiv :: "efsm \<Rightarrow> efsm \<Rightarrow> trace \<Rightarrow> bool" where
-"equiv e1 e2 t \<equiv> (observe e1 t) = (observe e2 t)"
+definition state_trace :: "transition_matrix \<Rightarrow> nat \<Rightarrow> datastate \<Rightarrow> trace \<Rightarrow> nat list" where
+  "state_trace e s r t \<equiv> map (\<lambda>(t,x,y,z). x) (observe_all e s r t)"
 
-lemma equiv_comute: "equiv e1 e2 t \<equiv> equiv e2 e1 t"
-  by (smt EFSM.equiv_def)
+definition transition_trace :: "transition_matrix \<Rightarrow> nat \<Rightarrow> datastate \<Rightarrow> trace \<Rightarrow> transition list" where
+  "transition_trace e s r t \<equiv> map (\<lambda>(t,x,y,z). t) (observe_all e s r t)"
 
-lemma equiv_trans: "equiv e1 e2 t \<and> equiv e2 e3 t \<longrightarrow> equiv e1 e3 t"
-  by (simp add: EFSM.equiv_def)
+definition efsm_equiv :: "transition_matrix \<Rightarrow> transition_matrix \<Rightarrow> trace \<Rightarrow> bool" where
+  "efsm_equiv e1 e2 t \<equiv> ((observe_trace e1 0 <> t) = (observe_trace e2 0 <> t))"
 
-lemma equiv_idem: "equiv e1 e1 t"
-  by (simp add: EFSM.equiv_def)
+lemma efsm_equiv_reflexive: "efsm_equiv e1 e1 t"
+  by (simp add: efsm_equiv_def)
 
+lemma efsm_equiv_symmetric: "efsm_equiv e1 e2 t \<equiv> efsm_equiv e2 e1 t"
+  apply (simp add: efsm_equiv_def)
+  by argo
+
+lemma efsm_equiv_transitive: "efsm_equiv e1 e2 t \<and> efsm_equiv e2 e3 t \<longrightarrow> efsm_equiv e1 e3 t"
+  by (simp add: efsm_equiv_def)
+
+lemmas observations = observe_trace_def step_def possible_steps_def
+
+lemma different_observation_techniques: "length(observe_all e s r t) = length(observe_trace e s r t)"
+  by (simp add: observe_trace_def)
+
+lemma length_observe_all_restricted: "\<And>s r. length (observe_all e s r t) \<le> length t"
+proof (induction t)
+  case Nil
+  then show ?case by simp
+next
+  case (Cons a t)
+  then show ?case
+  proof cases
+    assume "step e s r (fst a) (snd a) = None"
+    then show ?thesis by simp
+  next
+    assume "step e s r (fst a) (snd a) \<noteq>  None"
+    with Cons show ?thesis by(auto)
+  qed
+qed
+
+inductive accepts :: "transition_matrix \<Rightarrow> nat \<Rightarrow> datastate \<Rightarrow> trace \<Rightarrow> bool" where
+  base: "accepts e s d []" |
+  step: "step e s d (fst h) (snd h) = Some (tr, s', p', d') \<Longrightarrow> accepts e s' d' t \<Longrightarrow> accepts e s d (h#t)"
+
+definition accepts_trace :: "transition_matrix \<Rightarrow> trace \<Rightarrow> bool" where
+  "accepts_trace e t = accepts e 0 <> t"
+
+lemma no_step_none: "step e s r aa ba = None \<Longrightarrow> \<not>accepts e s r ((aa, ba) # p)"
+  apply safe
+  apply (rule accepts.cases)
+    apply simp
+   apply simp
+  by auto
+
+lemma accepts_steps: "fthe_elem (possible_steps e s d (fst h) (snd h)) = (a, b) \<Longrightarrow>
+       fis_singleton (possible_steps e s d (fst h) (snd h)) \<Longrightarrow>
+       accepts e a (apply_updates (Updates b) (case_vname (\<lambda>n. input2state (snd h) (Suc 0) (I n)) (\<lambda>n. d (R n))) d) t \<Longrightarrow>
+       accepts e s d (h#t)"
+  by (simp add: observations accepts.step)
+
+lemma inaccepts_conditions: "\<not>accepts e s d (h # t) \<Longrightarrow> step e s d (fst h) (snd h) = None \<or> (\<exists>tr s' p' d'. step e s d (fst h) (snd h) =  Some (tr, s', p', d') \<and> \<not>accepts e s' d' t)"
+  apply (rule accepts.cases)
+  using accepts.base
+    apply auto[1]
+   apply (metis option.exhaust prod_cases4 accepts.step)
+  by simp
+
+lemma step_none_inaccepts: "((step e s d (fst h) (snd h)) = None) \<Longrightarrow> \<not> (accepts e s d (h#t))"
+  apply(clarify)
+  apply(cases rule:accepts.cases)
+    apply(simp)
+   apply simp
+  by(auto)
+
+lemma inaccepts_future_inaccepts: "(\<exists>tr s' p' d'. step e s d (fst h) (snd h) =  Some (tr, s', p', d') \<and> \<not>accepts e s' d' t) \<Longrightarrow> \<not>accepts e s d (h#t)"
+  apply clarify
+    apply(cases rule: accepts.cases)
+    apply simp
+   apply simp
+  by auto
+
+lemma conditions_inaccepts: "step e s d (fst h) (snd h) = None \<or> (\<exists>tr s' p' d'. step e s d (fst h) (snd h) =  Some (tr, s', p', d') \<and> \<not>accepts e s' d' t) \<Longrightarrow> \<not> accepts e s d (h # t)"
+  apply clarify
+    apply(cases rule:accepts.cases)
+    apply simp
+   apply simp
+  by auto
+
+lemma accepts_head: "accepts e s d (h#t) \<Longrightarrow> accepts e s d [h]"
+  by (meson base conditions_inaccepts inaccepts_conditions)
+
+lemma inaccepts_single_event: "\<not> accepts e s d [(a, b)] \<Longrightarrow> step e s d (fst (a, b)) (snd (a, b)) = None"
+  by (metis (mono_tags, lifting) base inaccepts_conditions)
+
+lemma step_inaccepts: "\<not> accepts e s d ((a, b) # t) \<Longrightarrow> step e s d (fst (a, b)) (snd (a, b)) = Some (tr, s', p', d') \<Longrightarrow> \<not> accepts e s' d' t"
+  using inaccepts_conditions by force
+
+lemma step_none_inaccepts_append: "step e s d (fst a) (snd a) = None \<Longrightarrow> \<not>accepts e s d (a # t) \<and> \<not>accepts e s d (a # t @ t')"
+  by (simp add: step_none_inaccepts)
+
+lemma step_some: "step e s d (fst a) (snd a) = Some (tr, aa, ab, b) \<Longrightarrow> accepts e s d (a # t) = accepts e aa b t"
+  apply safe
+  using conditions_inaccepts apply fastforce
+  by (simp add: accepts.step)
+
+lemma aux1: "\<forall> s d. accepts e s d (t@t') \<longrightarrow> accepts e s d t"
+  proof (induction t)
+    case Nil
+    then show ?case by (simp add: base)
+  next
+    case (Cons a t)
+    then show ?case
+      apply safe
+      apply simp
+      apply (case_tac "step e s d (fst a) (snd a) = None")
+       apply (simp add: step_none_inaccepts)
+      apply safe
+      by (simp add: step_some)
+  qed
+
+lemma prefix_closure: "accepts e s d (t@t') \<Longrightarrow> accepts e s d t"
+  proof (induction "t")
+    case Nil
+    then show ?case by (simp add: base)
+  next
+    case (Cons x xs)
+    then show ?case
+      apply simp
+      apply (case_tac "step e s d (fst x) (snd x) = None")
+       apply (simp add: step_none_inaccepts)
+      apply safe
+      apply (simp add: step_some)
+      using aux1 by force
+  qed
+
+lemma inaccepts_prefix: "\<not>accepts e s d t \<Longrightarrow> \<not>accepts e s d (t@t')"
+  apply (rule ccontr)
+  by (simp add: prefix_closure)
+
+lemma length_observe_empty_trace: "length (observe_all e aa b []) = 0"
+  by simp
+
+lemma not_single_step_none:  "\<not> fis_singleton (possible_steps e 0 Map.empty (fst a) (snd a)) \<Longrightarrow> (step e 0 <> (fst a) (snd a) = None)"
+  by (simp add: observations)
+
+lemma accepts_singleton_first_step: "accepts e 0 Map.empty (a # t) \<Longrightarrow> fis_singleton (possible_steps e 0 Map.empty (fst a) (snd a))"
+  by (meson step_none_inaccepts observations)
+
+lemma step_length_suc: "step e 0 <> (fst a) (snd a) = Some (tr, aa, ab, b) \<Longrightarrow> length (observe_all e 0 <> (a # t)) = Suc (length (observe_all e aa b t))"
+  by simp
+
+lemma aux2: "\<forall>s d. accepts e s d t \<longrightarrow> (length t = length (observe_all e s d t))"
+  proof (induction t)
+    case Nil
+    then show ?case by simp
+  next
+    case (Cons a t)
+    then show ?case
+      apply safe
+      apply (simp add: step_def)
+      apply (case_tac "fthe_elem (possible_steps e s d (fst a) (snd a))")
+      apply simp
+      apply safe
+      using step_some observations
+       apply (simp add: step_some)
+      using step_none_inaccepts observations
+      by metis
+  qed
+
+lemma accepts_trace_obs_equal_length: "accepts e 0 <> t \<Longrightarrow> (length t = length (observe_all e 0 <> t))"
+  proof (induction t rule: accepts.induct)
+    case (base e s d)
+    then show ?case
+      by simp
+  next
+    case (step e s d h tr s' p' d' t)
+    then show ?case
+      by simp
+  qed
+
+lemma aux3: "\<forall>s d. (length t = length (observe_all e s d t)) \<longrightarrow> accepts e s d t"
+  proof (induction t)
+    case Nil
+    then show ?case by (simp add: accepts.base)
+  next
+    case (Cons a t)
+    then show ?case
+      apply safe
+      apply simp
+      apply (case_tac "step e s d (fst a) (snd a)")
+       apply simp
+      apply simp
+      apply (case_tac aa)
+      apply simp
+      by (simp only: step_length_suc step_some)
+  qed
+
+lemma obs_equal_length_accepts: "(length t = length (observe_all e 0 <> t)) \<Longrightarrow> accepts e 0 <> t"
+  proof (induction t)
+    case Nil
+    then show ?case by (simp add: accepts.base)
+  next
+    case (Cons a t)
+    then show ?case
+      apply (case_tac "step e 0 <> (fst a) (snd a) = None")
+       apply simp
+      apply (simp add: step_def)
+      apply (case_tac "fis_singleton (possible_steps e 0 Map.empty (fst a) (snd a))")
+      apply (case_tac "fthe_elem (possible_steps e 0 Map.empty (fst a) (snd a))")
+       apply simp
+      using observations aux3 apply fastforce
+      by simp
+  qed
+
+lemma length_equal_accepts: "(length t = length (observe_all e 0 <> t)) = accepts e 0 <> t"
+  apply safe
+  using obs_equal_length_accepts apply auto[1]
+  by (simp add: accepts_trace_obs_equal_length)
+
+type_synonym simulation_relation = "nat \<Rightarrow> nat"
+
+inductive simulates_trace :: "transition_matrix \<Rightarrow> transition_matrix \<Rightarrow> nat \<Rightarrow> nat \<Rightarrow> datastate \<Rightarrow> datastate \<Rightarrow> trace \<Rightarrow> bool" where
+  base: "simulates_trace e1 e2 s1 s2 d1 d2 []" |
+  step: "step e1 s1 d1 (fst h) (snd h) = Some (tr1, s1', p', d1') \<Longrightarrow>
+         step e2 s2 d2 (fst h) (snd h) = Some (tr2, s2', p', d2') \<Longrightarrow>
+         simulates_trace e1 e2 s1' s2' d1' d2' t \<Longrightarrow> simulates_trace e1 e2 s1 s2 d1 d2 (h#t)"
+
+definition simulates :: "transition_matrix \<Rightarrow> transition_matrix \<Rightarrow> bool" where
+  "simulates m1 m2 = (\<forall>t. simulates_trace m1 m2 0 0 <> <> t)"
+
+inductive gets_us_to :: "nat \<Rightarrow> transition_matrix \<Rightarrow> nat \<Rightarrow> datastate \<Rightarrow> trace \<Rightarrow> bool" where
+  base: "s = target \<Longrightarrow> gets_us_to target _ s _ []" |
+  step_some: "step e s r (fst h) (snd h) =  Some (_, s', _, r') \<Longrightarrow> gets_us_to target e s' r' t \<Longrightarrow> gets_us_to target e s r (h#t)" |
+  step_none: "step e s r (fst h) (snd h) = None \<Longrightarrow> s=target \<Longrightarrow> gets_us_to target e s r (h#t)"
+
+lemma no_further_steps: "s \<noteq> s' \<Longrightarrow> \<not> gets_us_to s e s' r []"
+  apply safe
+  apply (rule gets_us_to.cases)
+  by auto
 end
