formal/Lift.thy
@@ -1,7 +1,0 @@
-theory Lift
-  imports EFSM
-begin
-
-
-
-end
